standardise naming scheme using namespaces

src/examples/nat_fol.lean
@@ -2,93 +2,100 @@ import fol
 
 set_option pp.beta true
 
+namespace fol_nat
+
+open fol
+
 -- example 1a: A language of natural numbers with the constant symbols `zero` and `one`
 -- and the function symbols `succ` and `add`
-inductive natFuncs : ℕ → Type
-| zero : natFuncs 0
-| one : natFuncs 0
-| succ : natFuncs 1
-| add : natFuncs 2
+inductive funcs : ℕ → Type
+| zero : funcs 0
+| one : funcs 0
+| succ : funcs 1
+| add : funcs 2
 
-inductive natRels : ℕ → Type
-| equals : natRels 2
+inductive preds : ℕ → Type
+| equals : preds 2
 
-def natLanguage : Language := ⟨natFuncs, natRels⟩
+def L : language := ⟨funcs, preds⟩
 -- End Example
 
--- Example 1b: shorthand for each function/constant symbol in natLanguage of example 1a
-def zero : FOLTerm natLanguage := FOLTerm.func natFuncs.zero fin.empty
-def one : FOLTerm natLanguage := FOLTerm.func natFuncs.one fin.empty
-def succ (arg : FOLTerm natLanguage) : FOLTerm natLanguage := 
-FOLTerm.func natFuncs.succ (arg :: fin.empty)
-def add (arg1 arg2 : FOLTerm natLanguage) : FOLTerm natLanguage := 
-FOLTerm.func natFuncs.add (arg1 :: arg2 :: fin.empty)
-def equ (arg1 arg2 : FOLTerm natLanguage) : FOLPred natLanguage := 
-FOLPred.pred natRels.equals (arg1 :: arg2 :: fin.empty)
+-- Example 1b: shorthand for each function/constant symbol in L of example 1a
+def zero : term L := term.func funcs.zero fin.empty
+def one : term L := term.func funcs.one fin.empty
+def succ (arg : term L) : term L := 
+term.func funcs.succ (arg :: fin.empty)
+def add (arg1 arg2 : term L) : term L := 
+term.func funcs.add (arg1 :: arg2 :: fin.empty)
+def equ (arg1 arg2 : term L) : atom L := 
+atom.atom preds.equals (arg1 :: arg2 :: fin.empty)
 -- End Example
 
 -- Example 2a: model for the natural number language of example 1a
-def natFuncSemantics (n : ℕ) (c : natFuncs n) : (fin.vec n ℕ → ℕ) :=
+def interpret_func (n : ℕ) (c : funcs n) : (fin.vec n ℕ → ℕ) :=
 match n, c with
-| 0, natFuncs.zero := (λ_, 0)
-| 0, natFuncs.one  := (λ_, 1)
-| 1, natFuncs.succ := (λargs, args 0 + 1)
-| 2, natFuncs.add  := (λargs, args 0 + args 1)
+| 0, funcs.zero := (λ_, 0)
+| 0, funcs.one  := (λ_, 1)
+| 1, funcs.succ := (λargs, args 0 + 1)
+| 2, funcs.add  := (λargs, args 0 + args 1)
 end
 
-def natRelSemantics (n : ℕ) (c : natRels n) : (fin.vec n ℕ → Prop) :=
+def interpret_pred (n : ℕ) (c : preds n) : (fin.vec n ℕ → Prop) :=
 match n, c with
-| 2, natRels.equals := (λargs, args 0 = args 1)
+| 2, preds.equals := (λargs, args 0 = args 1)
 end
 
-def natModel : Model natLanguage :=
-{domain := ℕ, terms := natFuncSemantics, preds := natRelSemantics}
+def M : model L :=
+{domain := ℕ, funcs := interpret_func, preds := interpret_pred}
 -- End Example
 
 -- Example 2b: interpreting a ground term in the natural language using the natural model
-def interpretNatTerm (t : FOLTerm natLanguage) : ℕ :=
-termSemantics natModel (λi, nat.zero) t
+def interpret_term (t : term L) : ℕ :=
+term.valuation M (λi, nat.zero) t
 
-#reduce interpretNatTerm $ succ (add one one)
+#reduce interpret_term $ succ (add one one)
 
-example : interpretNatTerm (succ (add one one)) = 3 :=
+example : interpret_term (succ (add one one)) = 3 :=
 rfl
 -- End Example
 
 -- Example 2c: interpreting a ground predicate and proving the predicate
-def interpretNatPred (p : FOLPred natLanguage) : Prop :=
-predSemantics natModel (λi, nat.zero) p
+def interpret_atom (p : atom L) : Prop :=
+atom.valuation M (λi, nat.zero) p
 
-#reduce interpretNatPred $ equ one (succ zero)
+#reduce interpret_atom $ equ one (succ zero)
 
-example : interpretNatPred (equ one (succ zero)) ↔ (1 = 1) :=
+example : interpret_atom (equ one (succ zero)) ↔ (1 = 1) :=
 iff.rfl
 
-example : interpretNatPred (equ one (succ zero)) :=
+example : interpret_atom (equ one (succ zero)) :=
 rfl
 -- End Example
 
 -- Example 2d: interpreting some sentences and proving the sentences
-def interpretNatFormula (f : FOLFormula natLanguage) : Prop :=
-formulaSemantics natModel (λi, nat.zero) f
+def interpret_formula (f : formula L) : Prop :=
+formula.valuation M (λi, nat.zero) f
 
-def natRefl : FOLFormula natLanguage := 
-∀_(FOLFormula.pred $ equ (FOLTerm.var 0) (FOLTerm.var 0))
+def reflexivity : formula L := 
+∀_(A_ (equ (term.var 0) (term.var 0)))
 
-#reduce interpretNatFormula natRefl
+#reduce interpret_formula reflexivity
 
-example : interpretNatFormula natRefl :=
+example : interpret_formula reflexivity :=
 by {intro, exact rfl}
 
-def natSymm : FOLFormula natLanguage := 
-∀_∀_((FOLFormula.pred $ equ (FOLTerm.var 0) (FOLTerm.var 1))
-     _→_(FOLFormula.pred $ equ (FOLTerm.var 1) (FOLTerm.var 0)))
+def symmetry : formula L := 
+∀_∀_((A_ (equ (term.var 0) (term.var 1)))
+     _→_(A_ (equ (term.var 1) (term.var 0))))
 
-#reduce interpretNatFormula natSymm
+#reduce interpret_formula symmetry
 
-example : interpretNatFormula natSymm :=
+example : interpret_formula symmetry :=
 begin
 intros x y h,
 exact h.symm
 end
+
 -- End Example
+
+end fol_nat
