src/fol.lean
@@ -2,113 +2,115 @@ import utils.finvec
 
 set_option pp.beta true
 
+namespace fol
+
 -- Syntax of First-Order Logic
-structure Language : Type 1 :=
-(functions : ℕ → Type) (relations : ℕ → Type)
+structure language : Type 1 :=
+(funcs : ℕ → Type) (preds : ℕ → Type)
 
 -- First Order Terms
-inductive FOLTerm (L : Language) : Type
-| var  : ℕ → FOLTerm
-| func : ∀ {n : ℕ} (name : L.functions n) (args : fin.vec n FOLTerm), FOLTerm
+inductive term (L : language) : Type
+| var  : ℕ → term
+| func : ∀ {n : ℕ} (name : L.funcs n) (args : fin.vec n term), term
 
 -- First Order Formulas
-inductive FOLPred (L : Language) : Type
-| pred : ∀ {n : ℕ} (name : L.relations n) (args : fin.vec n (FOLTerm L)), FOLPred
+inductive atom (L : language) : Type
+| atom : ∀ {n : ℕ} (name : L.preds n) (args : fin.vec n (term L)), atom
 
-inductive FOLFormula (L : Language) : Type
-| bottom  : FOLFormula
-| top     : FOLFormula
-| pred    : FOLPred L → FOLFormula
-| eq      : FOLTerm L → FOLTerm L → FOLFormula
-| and     : FOLFormula → FOLFormula → FOLFormula
-| or      : FOLFormula → FOLFormula → FOLFormula
-| imply   : FOLFormula → FOLFormula → FOLFormula
-| not     : FOLFormula → FOLFormula
-| for_all : FOLFormula → FOLFormula
-| exist   : FOLFormula → FOLFormula
+inductive formula (L : language) : Type
+| bottom  : formula
+| top     : formula
+| atom    : atom L → formula
+| eq      : term L → term L → formula
+| and     : formula → formula → formula
+| or      : formula → formula → formula
+| imply   : formula → formula → formula
+| not     : formula → formula
+| for_all : formula → formula
+| exist   : formula → formula
 
-notation `⨯` := FOLFormula.bottom -- \cross
-notation `✓` := FOLFormula.top -- \check
-prefix `P_` : max := FOLFormula.pred
-infixr `_=_`: 88 := FOLFormula.eq
-infixr `_∧_`: 60 := FOLFormula.and
-infixr `_∨_`: 61 := FOLFormula.or
-infixr `_→_`: 62 := FOLFormula.imply
-prefix `!_`: max := FOLFormula.not
-prefix `∀_`: 110 := FOLFormula.for_all
-prefix `∃_`: 110 := FOLFormula.exist
+notation `⨯`      := formula.bottom -- \cross
+notation `✓`      := formula.top -- \check
+prefix `A_` : max := formula.atom
+infixr `_=_`: 88  := formula.eq
+infixr `_∧_`: 60  := formula.and
+infixr `_∨_`: 61  := formula.or
+infixr `_→_`: 62  := formula.imply
+prefix `!_`: max  := formula.not
+prefix `∀_`: 110  := formula.for_all
+prefix `∃_`: 110  := formula.exist
 
 -- bounded representations of terms and formulas such that the type carries
 -- a parameter n such that all *free* variables occuring in the term/formula
 -- are less than n.
 
-inductive FOLBoundedT (L : Language) : ℕ → Type
-| var  : ∀(i : ℕ), FOLBoundedT (i + 1)
-| func : ∀{n : ℕ} {f : fin n → ℕ} (name : L.functions n)
-         (args : fin.dvec n (λi, FOLBoundedT (f i))), 
-         FOLBoundedT (fin.max f)
+inductive bounded_term (L : language) : ℕ → Type
+| var  : ∀(i : ℕ), bounded_term (i + 1)
+| func : ∀{n : ℕ} {f : fin n → ℕ} (name : L.funcs n)
+         (args : fin.dvec n (λi, bounded_term (f i))), 
+         bounded_term (fin.max f)
 
-def FOLClosedTerm (L : Language) : Type := FOLBoundedT L 0
+def closed_term (L : language) : Type := bounded_term L 0
 
 -- Given an unbounded term, return a bound value k and a term bounded by k
-def FOLTerm.toBoundedT {L : Language} : FOLTerm L → Σ{k : ℕ}, FOLBoundedT L k
-| (FOLTerm.var i) := ⟨i + 1, FOLBoundedT.var i⟩
-| (FOLTerm.func name args) :=
-  let bArgs := (λi, (args i).toBoundedT) 
-  in ⟨fin.max $ fin.unzip_left bArgs, FOLBoundedT.func name (fin.unzip_right bArgs)⟩
+def term.to_bounded {L : language} : term L → Σ{k : ℕ}, bounded_term L k
+| (term.var i) := ⟨i + 1, bounded_term.var i⟩
+| (term.func name args) :=
+  let b_args := (λi, (args i).to_bounded) 
+  in ⟨fin.max $ fin.unzip_left b_args, bounded_term.func name (fin.unzip_right b_args)⟩
 
-inductive FOLBoundedP (L : Language) : ℕ → Type
-| pred : ∀{n : ℕ} {f : fin n → ℕ} (name : L.relations n)
-         (args : fin.dvec n (λi, FOLBoundedT L (f i))), 
-         FOLBoundedP (fin.max f)
+inductive bounded_atom (L : language) : ℕ → Type
+| atom : ∀{n : ℕ} {f : fin n → ℕ} (name : L.preds n)
+         (args : fin.dvec n (λi, bounded_term L (f i))), 
+         bounded_atom (fin.max f)
 
-def FOLClosedPred (L : Language) : Type := FOLBoundedP L 0
+def closed_atom (L : language) : Type := bounded_atom L 0
 
-def FOLPred.toBoundedP {L : Language} : FOLPred L → Σ{k : ℕ}, FOLBoundedP L k
-| (FOLPred.pred name args) := 
-  let b_args := (λi, (args i).toBoundedT)
-  in  ⟨fin.max $ fin.unzip_left b_args, FOLBoundedP.pred name (fin.unzip_right b_args)⟩
+def atom.to_bounded {L : language} : atom L → Σ{k : ℕ}, bounded_atom L k
+| (atom.atom name args) := 
+  let b_args := (λi, (args i).to_bounded)
+  in  ⟨fin.max $ fin.unzip_left b_args, bounded_atom.atom name (fin.unzip_right b_args)⟩
 
-inductive FOLBoundedF (L : Language) : ℕ → Type
-| bottom  : FOLBoundedF 0
-| top     : FOLBoundedF 0
-| pred    : ∀{n}, FOLBoundedP L n → FOLBoundedF n
-| eq      : ∀{n m}, FOLBoundedT L n → FOLBoundedT L m → FOLBoundedF (max n m)
-| and     : ∀{n m}, FOLBoundedF n → FOLBoundedF m → FOLBoundedF (max n m)
-| or      : ∀{n m}, FOLBoundedF n → FOLBoundedF m → FOLBoundedF (max n m)
-| imply   : ∀{n m}, FOLBoundedF n → FOLBoundedF m → FOLBoundedF (max n m)
-| not     : ∀{n}, FOLBoundedF n → FOLBoundedF n
-| for_all : ∀{n}, FOLBoundedF n → FOLBoundedF (n - 1)
-| exist   : ∀{n}, FOLBoundedF n → FOLBoundedF (n - 1)
+inductive bounded_formula (L : language) : ℕ → Type
+| bottom  : bounded_formula 0
+| top     : bounded_formula 0
+| atom    : ∀{n}, bounded_atom L n → bounded_formula n
+| eq      : ∀{n m}, bounded_term L n → bounded_term L m → bounded_formula (max n m)
+| and     : ∀{n m}, bounded_formula n → bounded_formula m → bounded_formula (max n m)
+| or      : ∀{n m}, bounded_formula n → bounded_formula m → bounded_formula (max n m)
+| imply   : ∀{n m}, bounded_formula n → bounded_formula m → bounded_formula (max n m)
+| not     : ∀{n}, bounded_formula n → bounded_formula n
+| for_all : ∀{n}, bounded_formula n → bounded_formula (n - 1)
+| exist   : ∀{n}, bounded_formula n → bounded_formula (n - 1)
 
-notation `:⨯` := FOLBoundedF.bottom -- \cross
-notation `:✓` := FOLBoundedF.top -- \check
-prefix `:P_` : max := FOLBoundedF.pred
-infixr `_:=_`: 88 := FOLBoundedF.eq
-infixr `_:∧_`: 60 := FOLBoundedF.and
-infixr `_:∨_`: 61 := FOLBoundedF.or
-infixr `_:→_`: 62 := FOLBoundedF.imply
-prefix `:!_`: max := FOLBoundedF.not
-prefix `:∀_`: 110 := FOLBoundedF.for_all
-prefix `:∃_`: 110 := FOLBoundedF.exist
+notation `:⨯`      := bounded_formula.bottom -- \cross
+notation `:✓`      := bounded_formula.top -- \check
+prefix `:A_` : max := bounded_formula.atom
+infixr `_:=_`: 88  := bounded_formula.eq
+infixr `_:∧_`: 60  := bounded_formula.and
+infixr `_:∨_`: 61  := bounded_formula.or
+infixr `_:→_`: 62  := bounded_formula.imply
+prefix `:!_`: max  := bounded_formula.not
+prefix `:∀_`: 110  := bounded_formula.for_all
+prefix `:∃_`: 110  := bounded_formula.exist
 
-def FOLFormula.toBoundedF {L : Language} : FOLFormula L → Σk : ℕ, FOLBoundedF L k
+def formula.to_bounded {L : language} : formula L → Σk : ℕ, bounded_formula L k
 | ⨯                   := ⟨0, :⨯⟩
 | ✓                   := ⟨0, :✓⟩
-| (FOLFormula.pred p) := let bp := p.toBoundedP in ⟨bp.fst, :P_ bp.snd⟩
-| (t₁ _=_ t₂)          := let bt₁ := t₁.toBoundedT, bt₂ := t₂.toBoundedT
+| (formula.atom p)    := let bp := p.to_bounded in ⟨bp.fst, :A_ bp.snd⟩
+| (t₁ _=_ t₂)          := let bt₁ := t₁.to_bounded, bt₂ := t₂.to_bounded
                          in  ⟨max bt₁.fst bt₂.fst, bt₁.snd _:=_ bt₂.snd⟩
-| (f₁ _∧_ f₂)          := let bf₁ := f₁.toBoundedF, bf₂ := f₂.toBoundedF
+| (f₁ _∧_ f₂)          := let bf₁ := f₁.to_bounded, bf₂ := f₂.to_bounded
                          in  ⟨max bf₁.fst bf₂.fst, bf₁.snd _:∧_ bf₂.snd⟩
-| (f₁ _∨_ f₂)          := let bf₁ := f₁.toBoundedF, bf₂ := f₂.toBoundedF
+| (f₁ _∨_ f₂)          := let bf₁ := f₁.to_bounded, bf₂ := f₂.to_bounded
                          in  ⟨max bf₁.fst bf₂.fst, bf₁.snd _:∨_ bf₂.snd⟩
-| (f₁ _→_ f₂)          := let bf₁ := f₁.toBoundedF, bf₂ := f₂.toBoundedF
+| (f₁ _→_ f₂)          := let bf₁ := f₁.to_bounded, bf₂ := f₂.to_bounded
                          in  ⟨max bf₁.fst bf₂.fst, bf₁.snd _:→_ bf₂.snd⟩
-| (!_ f)             := let bf := f.toBoundedF in ⟨bf.fst, :!_ bf.snd⟩
-| (∀_ f)             := let bf := f.toBoundedF in ⟨bf.fst - 1, :∀_ bf.snd⟩
-| (∃_ f)             := let bf := f.toBoundedF in ⟨bf.fst - 1, :∃_ bf.snd⟩
+| (!_ f)              := let bf := f.to_bounded in ⟨bf.fst, :!_ bf.snd⟩
+| (∀_ f)              := let bf := f.to_bounded in ⟨bf.fst - 1, :∀_ bf.snd⟩
+| (∃_ f)              := let bf := f.to_bounded in ⟨bf.fst - 1, :∃_ bf.snd⟩
 
-def FOLSentence (L : Language) : Type := FOLBoundedF L 0
+def sentence (L : language) : Type := bounded_formula L 0
 
 -- Semantics of First-Order Logic
 
@@ -116,34 +118,36 @@ def FOLSentence (L : Language) : Type := FOLBoundedF L 0
   * each function symbol (with arity n) in L as a mapping U^n → U
   * each relation symbol (with arity n) in L as a proposition over n arguments from U
   where U is the domain of the model -/
-structure Model (L : Language) :=
+structure model (L : language) :=
 (domain : Type)
-(terms : ∀ {n}, L.functions n → (fin.vec n domain → domain))
-(preds : ∀ {n}, L.relations n → (fin.vec n domain → Prop)) 
+(funcs : ∀ {n}, L.funcs n → (fin.vec n domain → domain))
+(preds : ∀ {n}, L.preds n → (fin.vec n domain → Prop)) 
 
-def termSemantics {L : Language} (m : Model L)
-                  (varSemantics : ℕ → m.domain) : FOLTerm L → m.domain
-| (FOLTerm.var n)           := varSemantics n
-| (FOLTerm.func name args) := (m.terms name) (λi, termSemantics (args i))
+def term.valuation {L : language} (m : model L)
+                  (var_assignment : ℕ → m.domain) : term L → m.domain
+| (term.var n)          := var_assignment n
+| (term.func name args) := (m.funcs name) (λi, term.valuation (args i))
 
-def predSemantics {L : Language} (m : Model L)
-                  (varSemantics : ℕ → m.domain) : FOLPred L → Prop
-| (FOLPred.pred name args) := (m.preds name) (λi, (termSemantics m varSemantics) (args i))
+def atom.valuation {L : language} (m : model L)
+                  (var_assignment : ℕ → m.domain) : atom L → Prop
+| (atom.atom name args) := (m.preds name) (λi, (term.valuation m var_assignment) (args i))
 
-def shift {L : Language} {m : Model L} 
-          (varSemantics : ℕ → m.domain) (x : m.domain) : (ℕ → m.domain)
+def shift {L : language} {m : model L} 
+          (var_assignment : ℕ → m.domain) (x : m.domain) : (ℕ → m.domain)
 | 0       := x
-| (n + 1) := varSemantics n
+| (n + 1) := var_assignment n
 
-def formulaSemantics {L : Language} (m : Model L) :
-                     (ℕ → m.domain) → FOLFormula L → Prop
+def formula.valuation {L : language} (m : model L) :
+                     (ℕ → m.domain) → formula L → Prop
 | vars ⨯ := false
 | vars ✓ := true
-| vars (FOLFormula.pred p) := predSemantics m vars p
-| vars (t₁ _=_ t₂) := (termSemantics m vars t₁) = (termSemantics m vars t₂)
-| vars (f₁ _∧_ f₂) := (formulaSemantics vars f₁) ∧ (formulaSemantics vars f₂)
-| vars (f₁ _∨_  f₂) := (formulaSemantics vars f₁) ∧ (formulaSemantics vars f₂)
-| vars (f₁ _→_ f₂) := (formulaSemantics vars f₁) → (formulaSemantics vars f₂)
-| vars (!_f) := ¬ (formulaSemantics vars f)
-| vars (∀_f) := ∀(x : m.domain), formulaSemantics (shift vars x) f
-| vars (∃_f) := ∃(x : m.domain), formulaSemantics (shift vars x) f
+| vars (formula.atom p) := atom.valuation m vars p
+| vars (t₁ _=_ t₂) := (term.valuation m vars t₁) = (term.valuation m vars t₂)
+| vars (f₁ _∧_ f₂) := (formula.valuation vars f₁) ∧ (formula.valuation vars f₂)
+| vars (f₁ _∨_  f₂) := (formula.valuation vars f₁) ∧ (formula.valuation vars f₂)
+| vars (f₁ _→_ f₂) := (formula.valuation vars f₁) → (formula.valuation vars f₂)
+| vars (!_f) := ¬ (formula.valuation vars f)
+| vars (∀_f) := ∀(x : m.domain), formula.valuation (shift vars x) f
+| vars (∃_f) := ∃(x : m.domain), formula.valuation (shift vars x) f
+
+end fol
