src/utils/finvec.lean
@@ -1,16 +1,18 @@
 import data.fin
 
-def fin.to_nat {n : ℕ} : fin n → ℕ := (fin.fin_to_nat n).coe
+namespace fin
 
-def fin.vec (n : ℕ) (U : Type) : Type := fin n → U
-def fin.dvec (n : ℕ) (U : fin n → Type) : Type := ∀(k : fin n), U k
+def to_nat {n : ℕ} : fin n → ℕ := (fin.fin_to_nat n).coe
 
-def fin.vec_to_dvec {n : ℕ} {U : Type} (v : fin.vec n U) : fin.dvec n (λ_, U) := v
+def vec (n : ℕ) (U : Type) : Type := fin n → U
+def dvec (n : ℕ) (U : fin n → Type) : Type := ∀(k : fin n), U k
 
-def fin.map {U V: Type} {n : ℕ} (f : U → V) (v : fin.vec n U) : fin.vec n V :=
+def vec_to_dvec {n : ℕ} {U : Type} (v : vec n U) : dvec n (λ_, U) := v
+
+def map {U V: Type} {n : ℕ} (f : U → V) (v : vec n U) : vec n V :=
 λi, f (v i)
 
-def fin.max' {n : ℕ} (vec : fin.vec (n + 1) ℕ) : fin (n + 1) → ℕ :=
+def max' {n : ℕ} (vec : vec (n + 1) ℕ) : fin (n + 1) → ℕ :=
 λfn, subtype.rec_on fn 
 (λm p, nat.rec_on m
   (vec 0) -- Base Case
@@ -18,22 +20,24 @@ def fin.max' {n : ℕ} (vec : fin.vec (n + 1) ℕ) : fin (n + 1) → ℕ :=
 )
 --The more readable version of max' but that causes timeouts when used for #reduce computation
 --| ⟨0, _⟩      := vec 0
---| ⟨k + 1, hk⟩ := max (vec (k + 1)) (fin.max' ⟨k, k.lt_succ_self.trans hk⟩)
+--| ⟨k + 1, hk⟩ := max (vec (k + 1)) (max' ⟨k, k.lt_succ_self.trans hk⟩)
 
-def fin.max {n : ℕ} : (fin.vec n ℕ) → ℕ :=
+def max {n : ℕ} : (vec n ℕ) → ℕ :=
 match n with
 | 0       := λv, 0
-| (k + 1) := λv, @fin.max' k v (fin.last k)
+| (k + 1) := λv, @max' k v (last k)
 end
 
-def fin.unzip_left {n : ℕ} {U : Type} {V : U → Type} (v : fin.vec n (Σx : U, V x)) 
-              : fin.vec n U :=
+def unzip_left {n : ℕ} {U : Type} {V : U → Type} (v : vec n (Σx : U, V x)) 
+              : vec n U :=
 λi, (v i).fst
 
-def fin.unzip_right {n : ℕ} {U : Type} {V : U → Type} (v : fin.vec n (Σx : U, V x)) 
-                    : fin.dvec n (V ∘ (fin.unzip_left v)) :=
+def unzip_right {n : ℕ} {U : Type} {V : U → Type} (v : vec n (Σx : U, V x)) 
+                    : dvec n (V ∘ (unzip_left v)) :=
 λi, (v i).snd
 
-def fin.empty {U : Type} : fin.vec 0 U := (λi, i.elim0)
+def empty {U : Type} : vec 0 U := (λi, i.elim0)
 
-infixr `::` := fin.cons
+infixr `::` := cons
+
+end fin
